\chapter{Proofs by Induction}
\section{Simple Induction}
\begin{wrapfigure}{l}{4cm}
  \begin{center}
    \vskip -0.5cm
    \qrset{link, height=3cm}
    \qrcode{https://youtu.be/jOnZTWGpX_I}
    \vskip 0.25cm
    \href{https://youtu.be/jOnZTWGpX_I}{youtu.be/jOnZTWGpX\_I}
  \end{center}
  \vskip -0.5cm
\end{wrapfigure}
Let us consider a simple problem: what is bigger $2^n$ or $n$? In this chapter
we are going to study the simplest way to prove that $2^n > n$ for all positive
integers $n$. Let us first prove it by contradiction. Assume that it is not
true; denote by $n_0$ the least positive integer such that $2^{n_0} \le n_0$.
We may consider the following two cases.
\begin{itemize}
  \item If $n_0 = 1$, then it leads to a contradiction since $2 = 2^1 > 1$.
  \item Otherwise, note that $1 \le n_0 - 1 < n_0$, hence,
    $2^{n_0 - 1} > n_0 - 1$. So $2^{n_0} > 2n_0 - 2 \ge n_0$. Which is a
    contradiction with the definition of $n_0$.
\end{itemize}

However, there is a problem in this approach, we have not explained why such
an $n_0$ exists.

In order to prove this statement formally, we use the following principle.
\begin{principle}[The Induction Principle]
  Let $P(n)$ be some statement about a positive integer $n$.
  Hence, $P(n)$ is true for every positive integer $n$ iff
  \begin{description}
    \item[base case:] $P(1)$ is true and
    \item[induction step:] $P(k) \implies P(k + 1)$ is true for all positive
      integers $k$.
  \end{description}
\end{principle}

Let's prove now the statement using this principle.
We define $P(n)$ be the statement that ``$2^n > n$''.
$P(1)$ is true since $2^1 > 1$. Let us assume now that $2^n > n$. Note that
$2^{n + 1} = 2 \cdot 2^n > 2n \ge n + 1$. Hence, we proved the induction step.

\begin{exercise}
  Prove that $(1 + x)^n \ge 1 + nx$ for all positive integers $n$ and real
  numbers $x \ge -1$.
\end{exercise}

\section{Changing the Base Case}
Let us consider functions $n^2$ and $2^n$.

\begin{center}
  \begin{tabular}{c | c | c | c | c | c | c | c | c}
    $n$   & 1 & 2 & 3 & 4  & 5  & 6  & 7   & 8   \\
    \hline
    $n^2$ & 1 & 4 & 9 & 16 & 25 & 36 & 49  & 64  \\
    $2^n$ & 2 & 4 & 8 & 16 & 32 & 64 & 128 & 256
  \end{tabular}
\end{center}
Note that $2^n$ is greater than $n^2$ starting from $5$. But without some trick
we can not prove this using induction since for $n = 3$ it is not true!

The trick is to use the statement $P(n)$ stating that $(n + 4)^2 < 2^{n + 4}$.
The base case when $n = 1$ is true.
Let us now prove the induction step. Assume that $P(k)$ is true i.e.
$(k + 4)^2 < 2^{k + 4}$. Note that $2(k + 4)^2 < 2^{k + 1 + 4}$ but
$(k + 5)^2 = k^2 + 10k + 25 \le 2k^2 + 8k + 32 = 2(k + 4)^2$. Which implies that
$2^{k + 1 + 4} > (k + 5)^2$. So $P(k + 1)$ is also true.

In order to avoid this strange $+4$ we may change the base
case and use the following argument.

\begin{theorem}
\label{theorem:induction-shifted-base}
  Let $P(n)$ be some statement about an integer $n$.
  Hence, $P(n)$ is true for every integer $n > n_0$ iff
  \begin{description}
    \item[base case:] $P(n_0 + 1)$ is true and
    \item[induction step:] $P(k) \implies P(k + 1)$ is true for all
      integers $k > n_0$.
  \end{description}
\end{theorem}

Using this generalized induction principle we may prove that $2^n \ge n^2$ for
$n \ge 5$. The base case for $n = 4$ is true. The induction step is also true;
indeed let $P(k)$ be true i.e. $(k + 4)^2 < 2^{k + 4}$. Hence,
$2(k + 4)^2 < 2^{k + 1 + 4}$ but
$(k + 5)^2 = k^2 + 10k + 25 \le 2k^2 + 8k + 32 = 2(k + 4)^2$.

Let us now prove the theorem. Note that the proof is based on an idea similar
to the trick with $+4$, we just used.
\begin{proof}[Proof of Theorem~\ref{theorem:induction-shifted-base}]
  \begin{description}
    \item[$\Rightarrow$] If $P(n)$ is true for any $n > n_0$ it is also true
      for $n = n_0 + 1$ which implies the base case. Additionally, it true for
      $n = k + 1$ so the induction step is also true.
    \item[$\Leftarrow$] In this direction the proof is a bit harder. Let us
      consider a statement $Q(n)$ saying that $P(n + n_0)$ is true. Note that
      by the base case for $P$, $Q(1)$ is true; by the induction step for $P$
      we know that $Q(n)$ implies $P(n + 1)$. As a result, by the induction
      principle $Q(n)$ is true for all positive integers $n$. Which implies
      that $P(n)$ is true for all integers $n > n_0$.
  \end{description}
\end{proof}

\section{Inductive Definitions}

We may also define objects inductively. Let us consider the sum
$1 + 2 + \dots + n$ a line of dots indicating ``and so on'' which indicates the
definition by induction. In this case a more precise notation is
$\sum_{i = 1}^n i$.

\begin{definition}
  Let $a(1)$, \dots, $a(n)$, \dots be a sequence of integers. Then
  $\sum_{i = 1}^n a(i)$ is defined inductively by the following
  statements:
  \begin{itemize}
    \item $\sum_{i = 1}^1 a(i) = a(1)$, and
    \item $\sum_{i = 1}^{k + 1} a(i) =
        \sum_{i = 1}^k a(i) + a(k + 1)$.
  \end{itemize}
\end{definition}

Let us prove that $\sum_{i = 1}^n i = \frac{n (n + 1)}{2}$.
Note that by definition $\sum_{i = 1}^1 i = 1$ and
$\frac{1 (1 + 1)}{2} = 1$; hence, the base case holds. Assume that
$\sum_{i = 1}^n i = \frac{n (n + 1)}{2}$. Note that
$\sum_{i = 1}^{n + 1} i = \sum_{i = 1}^n i + (n + 1)$ and by the
induction hypothesis $\sum_{i = 1}^n i = \frac{n (n + 1)}{2}$.
Hence, $\sum_{i = 1}^{n + 1} i = \frac{n (n + 1)}{2} + (n + 1) =
\frac{(n + 1)(n + 2)}{2}$.

\begin{exercise}
  Prove that $\sum_{i = 1}^n 2^i = 2^{n + 1} - 1$.
\end{exercise}

\section{Strong Induction}

Sometimes $P(k)$ is not enough to prove $P(k + 1)$ and we need all the
statements $P(1)$, \dots, $P(k)$. In this case we may use the following
induction  principle.

\begin{theorem}[The Strong Induction Principle]
\label{theorem:strong-induction}
  Let $P(n)$ be some statement about positive integer $n$.
  Hence, $P(n)$ is true for every integer $n > n_0$ iff
  \begin{description}
    \item[base case:] $P(n_0 + 1)$ is true and
    \item[induction step:] If $P(n_0 + 1)$, \dots, $P(n_0 + k)$ are true, then
      $P(n_0 + k + 1)$ is also true for all positive integers $k$.
  \end{description}
\end{theorem}

Before we prove this theorem let us prove some properties of Fibonacci numbers
using this theorem. The Fibonacci numbers are defined as follows:
$f_0 = 0$, $f_1 = 1$, and $f_k = f_{k - 1} + f_{k - 2}$ for $k \ge 3$.

\begin{theorem}[The Binet formula]
  The Fibonacci numbers are given by the following formula
  \[
      f_n = \frac{\alpha^n - \beta^n}{\sqrt{5}},
  \]
  where $\alpha = \frac{1 + \sqrt{5}}{2}$ and
  $\beta = \frac{1 - \sqrt{5}}{2}$.
\end{theorem}
\begin{proof}
  We use the strong induction principle to prove this statement with $n_0 = -1$.
  Let us first prove the base case,
  $\frac{(\alpha^0 - \beta^0)}{\sqrt{5}} = 0 = f_0$.
  We also need to prove the induction step.
  \begin{itemize}
    \item If $k = 1$, then $\frac{(\alpha^1 - \beta^1)}{\sqrt{5}} = 1 = f_1$.
    \item Otherwise, by the induction hypothesis,
      $f_k = \frac{\alpha^k - \beta^k}{\sqrt{5}}$ and
      $f_{k - 1} = \frac{\alpha^{k - 1} - \beta^{k - 1}}{\sqrt{5}}$.
      By the definition of the Fibonacci numbers $f_{k + 1} = f_k + f_{k - 1}$.
      Hence,
      \[
        f_{k + 1} = \frac{\alpha^k - \beta^k}{\sqrt{5}} +
        \frac{\alpha^{k - 1} - \beta^{k - 1}}{\sqrt{5}}.
      \]
      Note that it is enough to show that
      \begin{equation}
      \label{equation:binet}
        \frac{\alpha^{k + 1} - \beta^{k + 1}}{\sqrt{5}} =
        \frac{\alpha^k - \beta^k}{\sqrt{5}} +
        \frac{\alpha^{k - 1} - \beta^{k - 1}}{\sqrt{5}}.
      \end{equation}
      Note that it is the same as
      \[
        \frac{\alpha^{k + 1} - \alpha^k - \alpha^{k - 1}}{\sqrt{5}} =
        \frac{\beta^{k + 1} - \beta^k - \beta^{k - 1}}{\sqrt{5}}.
      \]
      Additionally, note that $\alpha$ and $\beta$ are roots of the equation
      $x^2 - x - 1 = 0$. Hence,
      $\alpha^{k + 1} - \alpha^k - \alpha^{k - 1} = \alpha^{k - 1}(\alpha^2 -
      \alpha - 1) = 0$ and
      $\beta^{k + 1} - \beta^k - \beta^{k - 1} =
      \beta^{k - 1}(\beta^2 - \beta - 1) = 0$. Which implies that
      equality~(\ref{equation:binet}).
  \end{itemize}
\end{proof}

Now we are ready to prove the strong induction principle.
\begin{proof}[Proof of Theorem~\ref{theorem:strong-induction}]
  It is easy to see that if $P(n)$ is true for all $n > n_0$, then the base
  case and the induction steps are true. Let us prove that if the base case and
  the induction step are true, then $P(n)$ is true for all $n > n_0$.

  Let $Q(k)$ be the statement that $P(n_0 + 1)$, \dots, $P(n_0 + k)$ are true.
  Note that $Q(1)$ is true by the base case for $P$. Additionally, note that if
  $Q(k)$ is true, then $Q(k + 1)$ is also true, by the induction step for $P$.
  Hence, by the induction principle, $Q(k)$ is true for all positive integers
  $k$. Which implies that $P(n_0 + k)$ is true for all positive integers $k$.
\end{proof}

\section{Recursive Definitions}
Sometimes you wish to define objects using objects of the same form like in the
case of inductive defenitions but you do not know how to enumerate them using
an integer parameter.

One example of such a situation is the definition of an arithmetic formula.
\begin{description}
  \item[base case:] $x_i$ is an arithmetic formula on the variables $x_1$,
    \dots, $x_n$ for all $i$.
  \item[recursion step:] If $P$ and $Q$ are arithmetic formulas on the variables
    $x_1$, \dots, $x_n$, then $(P + Q)$ and $P \cdot Q$ are arithmetic formulas
    on the variables $x_1$, \dots, $x_n$.
\end{description}
Note that this definition implicitly state that any other expressions are not
arithmetic formulas.

We can define recursively the value of such a formula. Let $v_1$, \dots, $v_n$
be some integers.
\begin{description}
  \item[base case:] $x_i\big\rvert_{x_1 = v_1, \dots, x_n = v_n} = v_i$; in other words,
    the value of the arythmetic formula $x_i$ is equal to $v_1$ when $x_1 =
    v_1$, \dots, $x_n = v_n$.
  \item[recursion step:] If $P$ and $Q$ are arythmetic formulas on the
    variables $x_1$, \dots, $x_n$, then
    \[
      (P + Q)\big\rvert_{x_1 = v_1, \dots, x_n = v_n} =
      P\big\rvert_{x_1 = v_1, \dots, x_n = v_n} + Q\big\rvert_{x_1 = v_1, \dots, x_n = v_n}
    \]
    and
    \[
      (P \cdot Q)\big\rvert_{x_1 = v_1, \dots, x_n = v_n} =
      P\big\rvert_{x_1 = v_1, \dots, x_n = v_n} \cdot Q\big\rvert_{x_1 = v_1, \dots, x_n = v_n}.
    \]
\end{description}

For example, $((x_1 + x_2) \cdot x_3)$ is clearly an arithmetic formula on the
variables $x_1$, \dots, $x_n$. One may expect the value of this formula with $x_1 = 1$, $x_2 = 0$, and $x_3 = -1$ be equal to $-1$, let us check:
\begin{itemize}
  \item Note that
    \[
      \begin{array}{l}
        x_1\big\rvert_{x_1 = 1, x_2 = 0, x_3 = -1} = 1, \\
        x_2\big\rvert_{x_1 = 1, x_2 = 0, x_3 = -1} = 0\text{, and} \\
        x_3\big\rvert_{x_1 = 1, x_2 = 0, x_3 = -1} = -1.
      \end{array}
    \]
  \item Hence,
    \[
      (x_1 + x_2)\big\rvert_{x_1 = 1, x_2 = 0, x_3 = -1} = 1 + 0 = 1.
    \]
  \item Finally,
    \[
      ((x_1 + x_2) \cdot x_3)\big\rvert_{x_1 = 1, x_2 = 0, x_3 = -1} = 1 \cdot -
      1 = -1.
    \]
\end{itemize}

\section*{End of The Chapter Exercises}
\begin{exercises}
  \exerciseitem Show that for any positive integer $n$, $n^2 + n$ is even.
  \exerciseitem Show that for any integer $n \ge 10$,
    $n^3 \le 2^n$.
  \exerciseitem Show that for any positive integer $n$,
    $\sum_{i = 0}^n x^i = \frac{1 - x^{n + 1}}{1 - x}$.
  \exerciseitem Show that for any matrix $A \in \mathbb{R}^{m \times n}$
    ($n > m$) there is a nonzero vector $x \in \mathbb{R}^n$ such that $Ax = 0$.
  \exerciseitem  Show that all the elements of $\set{0, 1}^n$ (Binary strings)
    may be ordered such that every successive strings in this order are
    different only in one character.
    (For example, for $n = 2$ the order may be $00$, $01$, $11$, $10$.)
  \exerciseitem Let $a_0 = 2$, $a_1 = 5$, and $a_n = 5a_{n - 1} - 6 a_{n - 2}$
    for all integers $n \ge 2$. Show that $a_n = 3^n + 2^n$ for all integers
    $n \ge 0$.
  \exerciseitem Show that $\sum_{i = 1}^n i^2 = \frac{n (n + 1)(2n + 1)}{6}$
    for all integers $n \ge 1$.
  \exerciseitem Show that $\sum\limits_{i = 1}^n \frac{1}{i (i + 1)} =
    \frac{n}{n + 1}$.
  \exerciseitem Let $f_0 = 1$, $f_1 = 1$, and $f_{n + 2} = f_{n + 1} + f_n$ for
    all $n \in \mathbb{N}$. Show that
    $f_n \ge \left(\frac{3}{2}\right)^{n - 2}$.
  \exerciseitem Show that $f_{n + m} = f_{n - 1} f_m + f_n f_{m + 1}$.
  \exerciseitem Show that two arythmetic formulas $(x_1 + x_2) \cdot x_3$ and
    $x_1 \cdot x_3 + x_2 \cdot x_3$ on the variables $x_1$, $x_2$, and $x_3$
    have the same values.
\end{exercises}
